@prefix :        <http://ont-loupe.linkeddata.es/def/core#> .
@prefix dc:      <http://purl.org/dc/elements/1.1/> .
@prefix rdfs:    <http://www.w3.org/2000/01/rdf-schema#> .
@prefix loupe:   <http://ont-loupe.linkeddata.es/def/core#> .
@prefix terms:   <http://purl.org/dc/terms/> .
@prefix owl:     <http://www.w3.org/2002/07/owl#> .
@prefix xsd:     <http://www.w3.org/2001/XMLSchema#> .
@prefix rdf:     <http://www.w3.org/1999/02/22-rdf-syntax-ns#> .
@prefix vann:    <http://purl.org/vocab/vann/> .
@prefix xml:     <http://www.w3.org/XML/1998/namespace> .
@prefix ontology:  <http://lexvo.org/ontology#> .

loupe:distinctSubjectCount
      a       owl:DatatypeProperty ;
      rdfs:comment "The total number of distinct subjects in a given collection of RDF triples."@en ;
      rdfs:label "distinctSubjectCount"@en ;
      rdfs:range xsd:long .

loupe:hasObjectType
      a       owl:ObjectProperty ;
      rdfs:domain loupe:TriplePatternPartition ;
      rdfs:label "hasObjectType"@en ;
      rdfs:range rdfs:Resource .

vann:preferredNamespaceUri
      a       owl:AnnotationProperty .

loupe:hasLanguagePattern
      a       owl:ObjectProperty ;
      rdfs:domain loupe:RDFDataset ;
      rdfs:label "hasLanguagePattern"@en ;
      rdfs:range loupe:LanguagePatternPartition .

loupe:DatatypePropertyPartition
      a       owl:Class ;
      rdfs:label "DatatypePropertyPartition"@en ;
      rdfs:subClassOf loupe:PropertyPartition .

loupe:LanguagePatternPartition
      a       owl:Class ;
      rdfs:label "LanguagePatternPartition"@en ;
      rdfs:subClassOf owl:Thing .

loupe:hasClassPropertyPartition
      a       owl:ObjectProperty ;
      rdfs:domain loupe:ClassPartition ;
      rdfs:range loupe:ClassPropertyPartition .

loupe:objectPropertyCount
      a       owl:DatatypeProperty ;
      rdfs:comment "The total number of distinct object properties used in a given collection of RDF triples."@en ;
      rdfs:label "objectPropertyCount"@en ;
      rdfs:range xsd:long ;
      rdfs:subPropertyOf loupe:propertyCount .

loupe:datatypePropertyCount
      a       owl:DatatypeProperty ;
      rdfs:comment "The total number of datatype properties in a given collection of RDF triples."@en ;
      rdfs:label "datatypePropertyCount"@en ;
      rdfs:range xsd:long ;
      rdfs:subPropertyOf loupe:propertyCount .

loupe:version
      a       owl:DatatypeProperty ;
      rdfs:comment "indicates the version of the dataset"@en ;
      rdfs:label "version"@en ;
      rdfs:range xsd:string .

loupe:aboutProperty
      a       owl:ObjectProperty ;
      rdfs:domain
              [ a       owl:Class ;
                owl:unionOf (loupe:ClassPropertyPartition loupe:PropertyPartition)
              ] ;
      rdfs:label "aboutProperty"@en ;
      rdfs:range rdf:Property .

owl:DatatypeProperty
      a       owl:Class ;
      rdfs:subClassOf rdf:Property .

dc:publisher
      a       owl:AnnotationProperty .

loupe:RDFDataset
      a       owl:Class ;
      rdfs:comment "An RDF dataset as defined by the the RDF 1.1 Concepts and Abstract Syntax W3C Recommendation, i.e., a collection of RDF graphs, and comprises."@en ;
      rdfs:label "RDFDataset"@en ;
      rdfs:subClassOf <http://www.w3.org/ns/dcat#Dataset> .

rdfs:Datatype
      a       owl:Class ;
      rdfs:subClassOf owl:Thing .

terms:license
      a       owl:AnnotationProperty .

loupe:hasPredicate
      a       owl:ObjectProperty ;
      rdfs:domain loupe:TriplePatternPartition ;
      rdfs:label "hasPredicate"@en ;
      rdfs:range rdf:Property .

loupe:OntologyElementPartition
      a       owl:Class ;
      rdfs:label "OntologyElementPartition"@en ;
      rdfs:subClassOf owl:Thing .

loupe:labelledEntityCount
      a       owl:DatatypeProperty ;
      rdfs:comment "The total number of entities (IRIs and blank nodes) with a label. For counting labels, we consider the properties rdfs:label. skos:prefLabel."@en ;
      rdfs:label "labelledEntityCount"@en ;
      rdfs:range xsd:long ;
      rdfs:subPropertyOf loupe:entityCount .

loupe:TriplePatternPartition
      a       owl:Class ;
      rdfs:label "TriplePatternPartition"@en .

<http://ont-loupe.linkeddata.es/def/core>
      a       owl:Ontology ;
      rdfs:comment "The Loupe ontology provides concepts and relations for describing the statistics about the triples, vocularies used, and common patterns observed in an RDF dataset."@en ;
      rdfs:label "Loupe Ontology"@en ;
      dc:publisher "http://oeg-upm.net" ;
      dc:title "Loupe ontology"@en ;
      terms:creator "http://purl.org/net/mpoveda"^^xsd:anyURI , "http://id.nandana.org/card#me"^^xsd:anyURI , "www.garcia-castro.com/foaf.rdf"^^xsd:anyURI ;
      terms:license <https://creativecommons.org/licenses/by/4.0/> ;
      vann:preferredNamespacePrefix
              "loupe" ;
      vann:preferredNamespaceUri
              "http://ont-loupe.linkeddata.es/def/core#" ;
      owl:versionInfo "0.1.1" .

owl:ObjectProperty
      a       owl:Class ;
      rdfs:subClassOf rdf:Property .

loupe:classSharingInstances
      a       owl:ObjectProperty ;
      rdfs:domain loupe:CommonInstancesPartition ;
      rdfs:label "classSharingInstances"@en ;
      rdfs:range rdfs:Class .

loupe:literalCount
      a       owl:DatatypeProperty ;
      rdfs:comment "The total number of distinct literals in a given collection of RDF triples."@en ;
      rdfs:label "literalCount"@en ;
      rdfs:range xsd:long ;
      rdfs:subPropertyOf loupe:entityCount .

loupe:aboutNamespace
      a       owl:ObjectProperty ;
      rdfs:domain loupe:VocabularyPartition ;
      rdfs:label "aboutNamespace"@en ;
      rdfs:range rdfs:Resource .

loupe:ClassPartition
      a       owl:Class ;
      rdfs:label "ClassPartition"@en ;
      rdfs:subClassOf loupe:OntologyElementPartition .

loupe:hasPropertyRangeDatatypePartition
      a       owl:ObjectProperty ;
      rdfs:domain loupe:DatatypePropertyPartition ;
      rdfs:range loupe:PropertyRangeDatatypePartition .

vann:preferredNamespacePrefix
      a       owl:AnnotationProperty .

loupe:blankSubjectCount
      a       owl:DatatypeProperty ;
      rdfs:comment "The total number of blank node subjects in a collection of triples."@en ;
      rdfs:label "blankSubjectCount"@en ;
      rdfs:range xsd:long .

loupe:hasNamedGraph
      a       owl:ObjectProperty ;
      rdfs:domain loupe:RDFDataset ;
      rdfs:label "hasNamedGraph"@en ;
      rdfs:range loupe:NamedGraph .

loupe:NamedGraph
      a       owl:Class ;
      rdfs:label "NamedGraph"@en ;
      rdfs:subClassOf owl:Thing .

loupe:langLabelledStringCount
      a       owl:DatatypeProperty ;
      rdfs:comment "The total number of string objects with a language tag in a given collection of RDF triples."@en ;
      rdfs:label "language labelled string count"@en ;
      rdfs:range xsd:long ;
      rdfs:subPropertyOf loupe:stringCount .

loupe:ObjectPropertyPartition
      a       owl:Class ;
      rdfs:label "ObjectPropertyPartition"@en ;
      rdfs:subClassOf loupe:PropertyPartition .

loupe:hasPropertyDomainPartition
      a       owl:ObjectProperty ;
      rdfs:domain loupe:PropertyPartition ;
      rdfs:range loupe:PropertyDomainPartition .

loupe:distinctObjectCount
      a       owl:DatatypeProperty ;
      rdfs:comment "The total number of distinct objects in a given collection of RDF triples."@en ;
      rdfs:label "distinctObjectCount"@en ;
      rdfs:range xsd:long .

loupe:PropertyDomainPartition
      a       owl:Class ;
      rdfs:label "PropertyDomainPartition"@en ;
      rdfs:subClassOf owl:Thing .

loupe:stringCount
      a       owl:DatatypeProperty ;
      rdfs:comment "The total number of string objects in a given collection of RDF triples."@en ;
      rdfs:label "stringCount"@en ;
      rdfs:range xsd:long ;
      rdfs:subPropertyOf loupe:literalCount .

loupe:includesClass
      a       owl:ObjectProperty ;
      rdfs:domain loupe:VocabularyPartition ;
      rdfs:label "includesClass"@en ;
      rdfs:range rdfs:Class .

loupe:hasCommonInstancesPartition
      a       owl:ObjectProperty ;
      rdfs:domain loupe:RDFDataset ;
      rdfs:label "hasCommonInstancesPartition"@en ;
      rdfs:range loupe:CommonInstancesPartition .

loupe:entityCount
      a       owl:DatatypeProperty ;
      rdfs:comment "The total number of distinct entities in a given collection of RDF triples. Entities are defined in the RDF 1.1 Concepts and Abstract Syntax W3C Recommendation as any IRI or literal that denotes something in the world. Anything can be an entity, including physical things, documents, abstract concepts, numbers and strings."@en ;
      rdfs:label "entityCount"@en ;
      rdfs:range xsd:long .

loupe:typedEntityCount
      a       owl:DatatypeProperty ;
      rdfs:label "typedEntityCount"@en ;
      rdfs:range xsd:long ;
      rdfs:subPropertyOf loupe:entityCount .

loupe:hasLanguage
      a       owl:ObjectProperty ;
      rdfs:domain loupe:RDFDataset ;
      rdfs:label "hasLanguage"@en ;
      rdfs:range ontology:Language .

loupe:hasElementPartition
      a       owl:ObjectProperty ;
      rdfs:domain loupe:RDFDataset ;
      rdfs:label "hasElementPartition"@en ;
      rdfs:range loupe:OntologyElementPartition ;
      owl:inverseOf loupe:usedInDataset .

loupe:aboutLanguage
      a       owl:ObjectProperty ;
      rdfs:domain loupe:LanguagePatternPartition ;
      rdfs:label "aboutLanguage"@en ;
      rdfs:range ontology:Language .

loupe:PropertyPartition
      a       owl:Class ;
      rdfs:label "PropertyPartition"@en ;
      rdfs:subClassOf loupe:OntologyElementPartition .

loupe:RDFDataProfile
      a       owl:Class ;
      rdfs:label "RDF Data Profile"@en ;
      rdfs:subClassOf loupe:RDFDataset .

loupe:datasetTripleCount
      a       owl:DatatypeProperty ;
      rdfs:domain rdfs:Datatype ;
      rdfs:label "datasetTripleCount"@en ;
      rdfs:range xsd:long ;
      rdfs:seeAlso <http://ont-loupe.linkeddata.es/def/core> ;
      rdfs:subPropertyOf loupe:tripleCount .

loupe:blankObjectCount
      a       owl:DatatypeProperty ;
      rdfs:comment "The total number of blank node objects in a collection of triples."@en ;
      rdfs:label "blankObjectCount"@en ;
      rdfs:range xsd:long .

loupe:PropertyRangeDatatypePartition
      a       owl:Class ;
      rdfs:label "PropertyRangeDatatypePartition"@en .

loupe:propertyCount
      a       owl:DatatypeProperty ;
      rdfs:comment "The total number of distinct properties used in a given collection of RDF triples."@en ;
      rdfs:label "propertyCount"@en ;
      rdfs:range xsd:long ;
      rdfs:subPropertyOf loupe:entityCount .

loupe:commonInstancesCount
      a       owl:DatatypeProperty ;
      rdfs:comment "The total count of common instances of given two classes in a collection of triples. The count is calculated using the explicit triples materialized in the collection without any inferencing. (e.g., if there is an instance x that is defined as \"x is an instance of Class A\" and \"x is an instance of Class B\", then x is counted as a common instance for class A and B.)"@en ;
      rdfs:domain loupe:CommonInstancesPartition ;
      rdfs:label "commonInstancesCount"@en ;
      rdfs:range xsd:long .

loupe:classCount
      a       owl:DatatypeProperty ;
      rdfs:comment "The total number of distinct RDFS or OWL classes utilized in a collection of triples."@en ;
      rdfs:label "classCount"@en ;
      rdfs:range xsd:long ;
      rdfs:subPropertyOf loupe:entityCount .

loupe:aboutNamedGraph
      a       owl:ObjectProperty ;
      rdfs:domain loupe:NamedGraph ;
      rdfs:label "aboutNamedGraph"@en ;
      rdfs:range rdfs:Resource .

loupe:includesProperty
      a       owl:ObjectProperty ;
      rdfs:domain loupe:VocabularyPartition ;
      rdfs:label "includesProperty"@en ;
      rdfs:range rdf:Property .

<http://www.w3.org/ns/dcat#Dataset>
      a       owl:Class .

dc:title
      a       owl:AnnotationProperty .

loupe:hasPropertyRangeClassPartition
      a       owl:ObjectProperty ;
      rdfs:domain loupe:ObjectPropertyPartition ;
      rdfs:range loupe:PropertyRangeClassPartition .

loupe:usedInDataset
      a       owl:ObjectProperty ;
      rdfs:domain loupe:OntologyElementPartition ;
      rdfs:label "usedInDataset"@en ;
      rdfs:range loupe:RDFDataset .

loupe:hasSubjectType
      a       owl:ObjectProperty ;
      rdfs:domain loupe:TriplePatternPartition ;
      rdfs:label "hasSubjectType"@en ;
      rdfs:range rdfs:Class .

loupe:VocabularyPartition
      a       owl:Class ;
      rdfs:label "VocabularyPartition"@en ;
      rdfs:subClassOf owl:Thing .

loupe:patternTripleCount
      a       owl:DatatypeProperty ;
      rdfs:comment "The total number of a triples conforming to a given abstract triple pattern."@en ;
      rdfs:domain loupe:TriplePatternPartition ;
      rdfs:label "patternTripleCount"@en ;
      rdfs:range xsd:long ;
      rdfs:subPropertyOf loupe:tripleCount .

rdfs:Resource
      a       owl:Class ;
      rdfs:subClassOf owl:Thing .

rdfs:Class
      a       owl:Class .

loupe:hasVocabularyPartition
      a       owl:ObjectProperty ;
      rdfs:domain loupe:RDFDataset ;
      rdfs:label "hasVocabularyPartition"@en ;
      rdfs:range loupe:VocabularyPartition .

ontology:Language
      a       owl:Class .

[]    a       owl:AllDisjointClasses ;
      owl:members (loupe:ClassPropertyPartition loupe:CommonInstancesPartition loupe:LanguagePatternPartition loupe:OntologyElementPartition loupe:PropertyDomainPartition loupe:PropertyRangeClassPartition loupe:PropertyRangeDatatypePartition loupe:RDFDataset loupe:TriplePatternPartition loupe:VocabularyPartition) .

loupe:graphTriplecount
      a       owl:DatatypeProperty ;
      rdfs:comment "The total number of triples in an RDF graph."@en ;
      rdfs:domain loupe:NamedGraph ;
      rdfs:label "graphTriplecount"@en ;
      rdfs:range xsd:long ;
      rdfs:subPropertyOf loupe:tripleCount .

loupe:tripleCount
      a       owl:DatatypeProperty ;
      rdfs:comment "The total number of triples in a collection of triples (e.g., RDF Dataset, or RDF Graph)."@en ;
      rdfs:label "tripleCount"@en ;
      rdfs:range xsd:long .

loupe:PropertyRangeClassPartition
      a       owl:Class ;
      rdfs:label "PropertyRangeClassPartition"@en ;
      rdfs:subClassOf owl:Thing .

loupe:CommonInstancesPartition
      a       owl:Class ;
      rdfs:label "CommonInstancesPartition"@en ;
      rdfs:subClassOf owl:Thing ;
      rdfs:subClassOf
              [ a       owl:Restriction ;
                owl:onClass rdfs:Class ;
                owl:onProperty loupe:classSharingInstances ;
                owl:qualifiedCardinality
                        "2"^^xsd:nonNegativeInteger
              ] .

rdf:Property
      a       owl:Class ;
      rdfs:subClassOf owl:Thing .

loupe:ClassPropertyPartition
      a       owl:Class ;
      rdfs:label "ClassPropertyPartition"@en .

loupe:instanceCount
      a       owl:DatatypeProperty ;
      rdfs:comment "The total number of instances of a given class."@en ;
      rdfs:subPropertyOf loupe:entityCount .

loupe:hasTriplePattern
      a       owl:ObjectProperty ;
      rdfs:domain loupe:RDFDataset ;
      rdfs:label "hasTriplePattern"@en ;
      rdfs:range loupe:TriplePatternPartition .

loupe:aboutClass
      a       owl:ObjectProperty ;
      rdfs:domain
              [ a       owl:Class ;
                owl:unionOf (loupe:ClassPartition loupe:PropertyDomainPartition loupe:PropertyRangeClassPartition)
              ] ;
      rdfs:label "aboutClass"@en ;
      rdfs:range rdfs:Class .

loupe:vocabularyCount
      a       owl:DatatypeProperty ;
      rdfs:comment "The total number of distinct vocabularies used in a givel collection of RDF triples either in a class declaration or as a property."@en ;
      rdfs:label "vocabularyCount"@en ;
      rdfs:range xsd:long .
