@prefix :        <http://ont-loupe.linkeddata.es/def/core#> .
@prefix dc:      <http://purl.org/dc/elements/1.1/> .
@prefix rdfs:    <http://www.w3.org/2000/01/rdf-schema#> .
@prefix terms:   <http://purl.org/dc/terms/> .
@prefix owl:     <http://www.w3.org/2002/07/owl#> .
@prefix xsd:     <http://www.w3.org/2001/XMLSchema#> .
@prefix rdf:     <http://www.w3.org/1999/02/22-rdf-syntax-ns#> .
@prefix vann:    <http://purl.org/vocab/vann/> .
@prefix xml:     <http://www.w3.org/XML/1998/namespace> .
@prefix core:    <http://ont-loupe.linkeddata.es/def/core#> .
@prefix ontology:  <http://lexvo.org/ontology#> .

core:distinctSubjectCount
      a       owl:DatatypeProperty ;
      rdfs:comment "The total number of distinct subjects in a given collection of RDF triples."@en ;
      rdfs:label "distinctSubjectCount"@en ;
      rdfs:range xsd:long .

core:hasObjectType
      a       owl:ObjectProperty ;
      rdfs:domain core:TriplePatternPartition ;
      rdfs:label "hasObjectType"@en ;
      rdfs:range rdfs:Resource .

vann:preferredNamespaceUri
      a       owl:AnnotationProperty .

core:hasLanguagePattern
      a       owl:ObjectProperty ;
      rdfs:domain core:RDFDataset ;
      rdfs:label "hasLanguagePattern"@en ;
      rdfs:range core:LanguagePatternPartition .

core:DatatypePropertyPartition
      a       owl:Class ;
      rdfs:label "DatatypePropertyPartition"@en ;
      rdfs:subClassOf core:PropertyPartition .

core:LanguagePatternPartition
      a       owl:Class ;
      rdfs:label "LanguagePatternPartition"@en ;
      rdfs:subClassOf owl:Thing .

core:hasClassPropertyPartition
      a       owl:ObjectProperty ;
      rdfs:domain core:ClassPartition ;
      rdfs:range core:ClassPropertyPartition .

core:objectPropertyCount
      a       owl:DatatypeProperty ;
      rdfs:comment "The total number of distinct object properties used in a given collection of RDF triples."@en ;
      rdfs:label "objectPropertyCount"@en ;
      rdfs:range xsd:long ;
      rdfs:subPropertyOf core:propertyCount .

core:datatypePropertyCount
      a       owl:DatatypeProperty ;
      rdfs:comment "The total number of datatype properties in a given collection of RDF triples."@en ;
      rdfs:label "datatypePropertyCount"@en ;
      rdfs:range xsd:long ;
      rdfs:subPropertyOf core:propertyCount .

core:version
      a       owl:DatatypeProperty ;
      rdfs:comment "indicates the version of the dataset"@en ;
      rdfs:label "version"@en ;
      rdfs:range xsd:string .

core:aboutProperty
      a       owl:ObjectProperty ;
      rdfs:domain
              [ a       owl:Class ;
                owl:unionOf (core:ClassPropertyPartition core:PropertyPartition)
              ] ;
      rdfs:label "aboutProperty"@en ;
      rdfs:range rdf:Property .

owl:DatatypeProperty
      a       owl:Class ;
      rdfs:subClassOf rdf:Property .

dc:publisher
      a       owl:AnnotationProperty .

core:RDFDataset
      a       owl:Class ;
      rdfs:comment "An RDF dataset as defined by the the RDF 1.1 Concepts and Abstract Syntax W3C Recommendation, i.e., a collection of RDF graphs, and comprises."@en ;
      rdfs:label "RDFDataset"@en ;
      rdfs:subClassOf <http://www.w3.org/ns/dcat#Dataset> .

rdfs:Datatype
      a       owl:Class ;
      rdfs:subClassOf owl:Thing .

terms:license
      a       owl:AnnotationProperty .

core:hasPredicate
      a       owl:ObjectProperty ;
      rdfs:domain core:TriplePatternPartition ;
      rdfs:label "hasPredicate"@en ;
      rdfs:range rdf:Property .

core:OntologyElementPartition
      a       owl:Class ;
      rdfs:label "OntologyElementPartition"@en ;
      rdfs:subClassOf owl:Thing .

core:labelledEntityCount
      a       owl:DatatypeProperty ;
      rdfs:comment "The total number of entities (IRIs and blank nodes) with a label. For counting labels, we consider the properties rdfs:label. skos:prefLabel."@en ;
      rdfs:label "labelledEntityCount"@en ;
      rdfs:range xsd:long ;
      rdfs:subPropertyOf core:entityCount .

core:TriplePatternPartition
      a       owl:Class ;
      rdfs:label "TriplePatternPartition"@en .

<http://ont-loupe.linkeddata.es/def/core>
      a       owl:Ontology ;
      rdfs:comment "The Loupe ontology provides concepts and relations for describing the statistics about the triples, vocularies used, and common patterns observed in an RDF dataset."@en ;
      rdfs:label "Loupe Ontology"@en ;
      dc:publisher "http://oeg-upm.net" ;
      dc:title "Loupe ontology"@en ;
      terms:creator "http://purl.org/net/mpoveda"^^xsd:anyURI , "http://id.nandana.org/card#me"^^xsd:anyURI , "www.garcia-castro.com/foaf.rdf"^^xsd:anyURI ;
      terms:license <http://www.apache.org/licenses/LICENSE-2.0> ;
      vann:preferredNamespacePrefix
              "loupe" ;
      vann:preferredNamespaceUri
              "http://ont-loupe.linkeddata.es/def/core#" ;
      owl:versionInfo "0.1.1" .

owl:ObjectProperty
      a       owl:Class ;
      rdfs:subClassOf rdf:Property .

core:classSharingInstances
      a       owl:ObjectProperty ;
      rdfs:domain core:CommonInstancesPartition ;
      rdfs:label "classSharingInstances"@en ;
      rdfs:range rdfs:Class .

core:literalCount
      a       owl:DatatypeProperty ;
      rdfs:comment "The total number of distinct literals in a given collection of RDF triples."@en ;
      rdfs:label "literalCount"@en ;
      rdfs:range xsd:long ;
      rdfs:subPropertyOf core:entityCount .

core:aboutNamespace
      a       owl:ObjectProperty ;
      rdfs:domain core:VocabularyPartition ;
      rdfs:label "aboutNamespace"@en ;
      rdfs:range rdfs:Resource .

core:ClassPartition
      a       owl:Class ;
      rdfs:label "ClassPartition"@en ;
      rdfs:subClassOf core:OntologyElementPartition .

core:hasPropertyRangeDatatypePartition
      a       owl:ObjectProperty ;
      rdfs:domain core:DatatypePropertyPartition ;
      rdfs:range core:PropertyRangeDatatypePartition .

vann:preferredNamespacePrefix
      a       owl:AnnotationProperty .

core:blankSubjectCount
      a       owl:DatatypeProperty ;
      rdfs:comment "The total number of blank node subjects in a collection of triples."@en ;
      rdfs:label "blankSubjectCount"@en ;
      rdfs:range xsd:long .

core:hasNamedGraph
      a       owl:ObjectProperty ;
      rdfs:domain core:RDFDataset ;
      rdfs:label "hasNamedGraph"@en ;
      rdfs:range core:NamedGraph .

core:NamedGraph
      a       owl:Class ;
      rdfs:label "NamedGraph"@en ;
      rdfs:subClassOf owl:Thing .

core:langLabelledStringCount
      a       owl:DatatypeProperty ;
      rdfs:comment "The total number of string objects with a language tag in a given collection of RDF triples."@en ;
      rdfs:label "language labelled string count"@en ;
      rdfs:range xsd:long ;
      rdfs:subPropertyOf core:stringCount .

core:ObjectPropertyPartition
      a       owl:Class ;
      rdfs:label "ObjectPropertyPartition"@en ;
      rdfs:subClassOf core:PropertyPartition .

core:hasPropertyDomainPartition
      a       owl:ObjectProperty ;
      rdfs:domain core:PropertyPartition ;
      rdfs:range core:PropertyDomainPartition .

core:distinctObjectCount
      a       owl:DatatypeProperty ;
      rdfs:comment "The total number of distinct objects in a given collection of RDF triples."@en ;
      rdfs:label "distinctObjectCount"@en ;
      rdfs:range xsd:long .

core:PropertyDomainPartition
      a       owl:Class ;
      rdfs:label "PropertyDomainPartition"@en ;
      rdfs:subClassOf owl:Thing .

core:stringCount
      a       owl:DatatypeProperty ;
      rdfs:comment "The total number of string objects in a given collection of RDF triples."@en ;
      rdfs:label "stringCount"@en ;
      rdfs:range xsd:long ;
      rdfs:subPropertyOf core:literalCount .

core:includesClass
      a       owl:ObjectProperty ;
      rdfs:domain core:VocabularyPartition ;
      rdfs:label "includesClass"@en ;
      rdfs:range rdfs:Class .

core:hasCommonInstancesPartition
      a       owl:ObjectProperty ;
      rdfs:domain core:RDFDataset ;
      rdfs:label "hasCommonInstancesPartition"@en ;
      rdfs:range core:CommonInstancesPartition .

core:entityCount
      a       owl:DatatypeProperty ;
      rdfs:comment "The total number of distinct entities in a given collection of RDF triples. Entities are defined in the RDF 1.1 Concepts and Abstract Syntax W3C Recommendation as any IRI or literal that denotes something in the world. Anything can be an entity, including physical things, documents, abstract concepts, numbers and strings."@en ;
      rdfs:label "entityCount"@en ;
      rdfs:range xsd:long .

core:typedEntityCount
      a       owl:DatatypeProperty ;
      rdfs:label "typedEntityCount"@en ;
      rdfs:range xsd:long ;
      rdfs:subPropertyOf core:entityCount .

core:hasLanguage
      a       owl:ObjectProperty ;
      rdfs:domain core:RDFDataset ;
      rdfs:label "hasLanguage"@en ;
      rdfs:range ontology:Language .

core:hasElementPartition
      a       owl:ObjectProperty ;
      rdfs:domain core:RDFDataset ;
      rdfs:label "hasElementPartition"@en ;
      rdfs:range core:OntologyElementPartition ;
      owl:inverseOf core:usedInDataset .

core:aboutLanguage
      a       owl:ObjectProperty ;
      rdfs:domain core:LanguagePatternPartition ;
      rdfs:label "aboutLanguage"@en ;
      rdfs:range ontology:Language .

core:PropertyPartition
      a       owl:Class ;
      rdfs:label "PropertyPartition"@en ;
      rdfs:subClassOf core:OntologyElementPartition .

core:datasetTripleCount
      a       owl:DatatypeProperty ;
      rdfs:domain rdfs:Datatype ;
      rdfs:label "datasetTripleCount"@en ;
      rdfs:range xsd:long ;
      rdfs:seeAlso <http://ont-loupe.linkeddata.es/def/core> ;
      rdfs:subPropertyOf core:tripleCount .

core:blankObjectCount
      a       owl:DatatypeProperty ;
      rdfs:comment "The total number of blank node objects in a collection of triples."@en ;
      rdfs:label "blankObjectCount"@en ;
      rdfs:range xsd:long .

core:PropertyRangeDatatypePartition
      a       owl:Class ;
      rdfs:label "PropertyRangeDatatypePartition"@en .

core:propertyCount
      a       owl:DatatypeProperty ;
      rdfs:comment "The total number of distinct properties used in a given collection of RDF triples."@en ;
      rdfs:label "propertyCount"@en ;
      rdfs:range xsd:long ;
      rdfs:subPropertyOf core:entityCount .

core:commonInstancesCount
      a       owl:DatatypeProperty ;
      rdfs:comment "The total count of common instances of given two classes in a collection of triples. The count is calculated using the explicit triples materialized in the collection without any inferencing. (e.g., if there is an instance x that is defined as \"x is an instance of Class A\" and \"x is an instance of Class B\", then x is counted as a common instance for class A and B.)"@en ;
      rdfs:domain core:CommonInstancesPartition ;
      rdfs:label "commonInstancesCount"@en ;
      rdfs:range xsd:long .

[]    a       owl:AllDisjointClasses ;
      owl:members (core:ClassPropertyPartition core:CommonInstancesPartition core:LanguagePatternPartition core:OntologyElementPartition core:PropertyDomainPartition core:PropertyRangeClassPartition core:PropertyRangeDatatypePartition core:RDFDataset core:TriplePatternPartition core:VocabularyPartition) .

core:classCount
      a       owl:DatatypeProperty ;
      rdfs:comment "The total number of distinct RDFS or OWL classes utilized in a collection of triples."@en ;
      rdfs:label "classCount"@en ;
      rdfs:range xsd:long ;
      rdfs:subPropertyOf core:entityCount .

core:aboutNamedGraph
      a       owl:ObjectProperty ;
      rdfs:domain core:NamedGraph ;
      rdfs:label "aboutNamedGraph"@en ;
      rdfs:range rdfs:Resource .

core:includesProperty
      a       owl:ObjectProperty ;
      rdfs:domain core:VocabularyPartition ;
      rdfs:label "includesProperty"@en ;
      rdfs:range rdf:Property .

<http://www.w3.org/ns/dcat#Dataset>
      a       owl:Class .

dc:title
      a       owl:AnnotationProperty .

core:hasPropertyRangeClassPartition
      a       owl:ObjectProperty ;
      rdfs:domain core:ObjectPropertyPartition ;
      rdfs:range core:PropertyRangeClassPartition .

core:usedInDataset
      a       owl:ObjectProperty ;
      rdfs:domain core:OntologyElementPartition ;
      rdfs:label "usedInDataset"@en ;
      rdfs:range core:RDFDataset .

core:hasSubjectType
      a       owl:ObjectProperty ;
      rdfs:domain core:TriplePatternPartition ;
      rdfs:label "hasSubjectType"@en ;
      rdfs:range rdfs:Class .

core:VocabularyPartition
      a       owl:Class ;
      rdfs:label "VocabularyPartition"@en ;
      rdfs:subClassOf owl:Thing .

core:patternTripleCount
      a       owl:DatatypeProperty ;
      rdfs:comment "The total number of a triples conforming to a given abstract triple pattern."@en ;
      rdfs:domain core:TriplePatternPartition ;
      rdfs:label "patternTripleCount"@en ;
      rdfs:range xsd:long ;
      rdfs:subPropertyOf core:tripleCount .

rdfs:Resource
      a       owl:Class ;
      rdfs:subClassOf owl:Thing .

rdfs:Class
      a       owl:Class .

core:hasVocabularyPartition
      a       owl:ObjectProperty ;
      rdfs:domain core:RDFDataset ;
      rdfs:label "hasVocabularyPartition"@en ;
      rdfs:range core:VocabularyPartition .

ontology:Language
      a       owl:Class .

core:graphTriplecount
      a       owl:DatatypeProperty ;
      rdfs:comment "The total number of triples in an RDF graph."@en ;
      rdfs:domain core:NamedGraph ;
      rdfs:label "graphTriplecount"@en ;
      rdfs:range xsd:long ;
      rdfs:subPropertyOf core:tripleCount .

core:tripleCount
      a       owl:DatatypeProperty ;
      rdfs:comment "The total number of triples in a collection of triples (e.g., RDF Dataset, or RDF Graph)."@en ;
      rdfs:label "tripleCount"@en ;
      rdfs:range xsd:long .

core:PropertyRangeClassPartition
      a       owl:Class ;
      rdfs:label "PropertyRangeClassPartition"@en ;
      rdfs:subClassOf owl:Thing .

core:CommonInstancesPartition
      a       owl:Class ;
      rdfs:label "CommonInstancesPartition"@en ;
      rdfs:subClassOf owl:Thing ;
      rdfs:subClassOf
              [ a       owl:Restriction ;
                owl:onClass rdfs:Class ;
                owl:onProperty core:classSharingInstances ;
                owl:qualifiedCardinality
                        "2"^^xsd:nonNegativeInteger
              ] .

rdf:Property
      a       owl:Class ;
      rdfs:subClassOf owl:Thing .

core:ClassPropertyPartition
      a       owl:Class ;
      rdfs:label "ClassPropertyPartition"@en .

core:instanceCount
      a       owl:DatatypeProperty ;
      rdfs:comment "The total number of instances of a given class."@en ;
      rdfs:subPropertyOf core:entityCount .

core:hasTriplePattern
      a       owl:ObjectProperty ;
      rdfs:domain core:RDFDataset ;
      rdfs:label "hasTriplePattern"@en ;
      rdfs:range core:TriplePatternPartition .

core:aboutClass
      a       owl:ObjectProperty ;
      rdfs:domain
              [ a       owl:Class ;
                owl:unionOf (core:ClassPartition core:PropertyDomainPartition core:PropertyRangeClassPartition)
              ] ;
      rdfs:label "aboutClass"@en ;
      rdfs:range rdfs:Class .

core:vocabularyCount
      a       owl:DatatypeProperty ;
      rdfs:comment "The total number of distinct vocabularies used in a givel collection of RDF triples either in a class declaration or as a property."@en ;
      rdfs:label "vocabularyCount"@en ;
      rdfs:range xsd:long .
